completing upd_reg

codeTest/correct_upd_reg.v
@@ -1,10 +1,10 @@
-From dx.tests Require Import DxIntegers DxValues DxMemRegion DxState DxMonad DxInstructions.
-From Coq Require Import List.
+From dx.tests Require Import DxIntegers DxValues DxMemRegion DxRegs DxState DxMonad DxInstructions.
+From Coq Require Import List Lia.
 From compcert Require Import Integers Values Clight Memory.
 Import ListNotations.
 Require Import ZArith.
 
-From bpf.proof Require Import Clightlogic MatchState CommonLemma interpreter.
+From bpf.proof Require Import Clightlogic MatchState CorrectRel CommonLemma interpreter.
 
 (**
 static void upd_reg (struct bpf_state* st, unsigned int i, unsigned long long v){
@@ -14,26 +14,24 @@ static void upd_reg (struct bpf_state* st, unsigned int i, unsigned long long v)
 Definition upd_reg (r: reg) (v: val64_t) : M unit := fun st => Some (tt, upd_reg r v st).
  *)
 
-Definition reg_correct (x:int64_t) (v: val) (stm:stateM) (m: Memory.Mem.mem) :=
-  Vlong x = v.
 
-Section Upd_pc.
+Section Upd_reg.
 
   (** The program contains our function of interest [fn] *)
   Definition p : Clight.program := prog.
 
   (* [Args,Res] provides the mapping between the Coq and the C types *)
   (* Definition Args : list CompilableType := [stateCompilableType].*)
-  Definition args : list Type := [(int64_t:Type)].
+  Definition args : list Type := [(reg:Type);val64_t].
   Definition res : Type := unit.
 
   (* [f] is a Coq Monadic function with the right type *)
-  Definition f : arrow_type args (M res) := DxMonad.upd_pc.
+  Definition f : arrow_type args (M res) := DxMonad.upd_reg.
 
   Variable state_block: block. (**r a block storing all rbpf state information? *)
 
   (* [fn] is the Cligth function which has the same behaviour as [f] *)
-  Definition fn: Clight.function := f_upd_pc.
+  Definition fn: Clight.function := f_upd_reg.
 
   Definition modifies : list block := [state_block]. (* of the C code *)
 
@@ -42,30 +40,38 @@ Section Upd_pc.
 
   (* [match_arg] relates the Coq arguments and the C arguments *)
   Definition match_arg_list : DList.t (fun x => x -> val -> stateM -> Memory.Mem.mem -> Prop) ((unit:Type) ::args) :=
-    DList.DCons stateM_correct (DList.DCons int64_correct (DList.DNil _)).
+    DList.DCons stateM_correct
+      (DList.DCons reg_correct
+        (DList.DCons (stateless val64_correct)
+          (DList.DNil _))).
 
   (* [match_res] relates the Coq result and the C result *)
   Definition match_res : res -> val -> stateM -> Memory.Mem.mem -> Prop := fun _ _ _ _ => True.
 
-  Lemma correct_function3_upd_pc : correct_function3 p args res f fn modifies false match_arg_list match_res.
+  Instance correct_function3_upd_reg : correct_function3 p args res f fn modifies false match_arg_list match_res.
   Proof.
     correct_function_from_body.
     correct_body.
     repeat intro.
     unfold INV in H.
     get_invariant_more _st.
-    get_invariant_more _pc.
+    get_invariant_more _i.
+    get_invariant_more _v.
     unfold stateM_correct in H1.
-    unfold int64_correct in H3.
+    unfold reg_correct in H3.
+    unfold stateless, val64_correct in H5.
     destruct H1 as (Hv_eq & Hst).
-    (*pose (mpc_store state_block st m Hst c (bpf_m st)). *)   
-    subst v0 v.
+    destruct H5 as (Hc_eq & (vl & Hvl_eq)).
+    subst v0 v v1 c0.
 
     simpl in c.
+    apply (upd_regs_store m _ _ c vl) in Hst as Hstore.
+    destruct Hstore as (m1 & Hstore).
+
     (**according to the type:
          static void upd_reg (struct bpf_state* st, unsigned int i, unsigned long long v)
        1. return value should be Vundef (i.e. void)
-       2. the new memory should change the value of pc, i.e. m_pc
+       2. the new memory should change the value of reg, i.e. m_reg
       *)
     exists Vundef, m1, Events.E0.
 
@@ -75,15 +81,17 @@ Section Upd_pc.
       repeat forward_plus.
 
       eapply Smallstep.plus_left'; eauto.
-      eapply step_assign; [do 4 econstructor; eauto | econstructor; eauto | econstructor; eauto| ..]. econstructor; eauto; reflexivity. (*
-        * do 4 econstructor; eauto. (**r how to do automatically in Ltac? *)
-        * econstructor; eauto.
-        * econstructor; eauto.
-        * econstructor; eauto; reflexivity.*)
+      repeat (econstructor; eauto; try deref_loc_tactic).
+      unfold Coqlib.align; simpl.
+      rewrite Ptrofs.add_zero_l.
+      assert (Heq: (8 + 8 * id_of_reg c)%Z = (Ptrofs.unsigned (Ptrofs.add (Ptrofs.repr 8) (Ptrofs.mul (Ptrofs.repr 8) (Ptrofs.of_intu (Int.repr (id_of_reg c))))))). {
+        unfold Ptrofs.add, Ptrofs.mul.
+        unfold id_of_reg; destruct c; try unfold Ptrofs.of_intu, Ptrofs.of_int; repeat rewrite Ptrofs.unsigned_repr; try rewrite Int.unsigned_repr; try rewrite Int_max_unsigned_eq64; try rewrite Ptrofs_max_unsigned_eq64; try lia.
+      }
+      rewrite <- Heq.
+      rewrite <- Hstore; reflexivity.
       forward_plus.
-      eapply Smallstep.plus_one; eauto.
-      eapply step_return_0.
-      reflexivity.
+      forward_plus.
       reflexivity.
     - simpl.
       constructor.
@@ -100,4 +108,6 @@ Section Upd_pc.
       left; assumption.
 Qed.
 
-End Upd_pc.
+End Upd_reg.
+
+Existing Instance correct_function3_upd_reg.
